AwsCryptographicMaterialProviders/dafny/AwsCryptographyKeyStoreAdmin/src/AwsCryptographyKeyStoreAdminOperations.dfy
@@ -1,0 +1,131 @@
+// Copyright Amazon.com Inc. or its affiliates. All Rights Reserved.
+// SPDX-License-Identifier: Apache-2.0
+include "../Model/AwsCryptographyKeyStoreAdminTypes.dfy"
+// include "../../AwsCryptographyKeyStore/src/AwsCryptographyKeyStoreOperations.dfy"
+// include "../../AwsCryptographicMaterialProviders/src/Keyrings/AwsKms/AwsKmsUtils.dfy"
+
+// include "GetKeys.dfy"
+// include "CreateKeyStoreTable.dfy"
+// include "CreateKeys.dfy"
+// include "Structure2.dfy"
+// include "ErrorMessages.dfy"
+// include "KmsArn.dfy"
+// include "DefaultEncryptedKeyStore.dfy"
+
+module AwsCryptographyKeyStoreAdminOperations refines AbstractAwsCryptographyKeyStoreAdminOperations {
+  import opened AwsKmsUtils
+  import KO = KMSKeystoreOperations
+  import KMS = ComAmazonawsKmsTypes
+  import DDB = ComAmazonawsDynamodbTypes
+  import MPL = AwsCryptographyMaterialProvidersTypes
+  import CreateKeys
+  import CreateKeyStoreTable
+  import GetKeys
+  import UUID
+  import Time
+  import Structure2
+  import ErrorMessages = KeyStoreErrorMessages
+  import KmsArn
+  import DefaultEncryptedKeyStore
+
+  import KeyStoreOperations = AwsCryptographyKeyStoreOperations
+  import KeyStoreTypes = KeyStoreOperations.Types
+
+  datatype Config = Config(
+    // nameonly id: string,
+    // nameonly ddbTableName: Option<DDB.TableName>,
+    nameonly logicalKeyStoreName: string,
+    // nameonly kmsConfiguration: KMSConfiguration,
+    // nameonly grantTokens: KMS.GrantTokenList,
+    // nameonly kmsClient: ComAmazonawsKmsTypes.IKMSClient,
+    // nameonly ddbClient: Option<ComAmazonawsDynamodbTypes.IDynamoDBClient>,
+    nameonly storage: KeyStoreTypes.IEncryptedKeyStore,
+    nameonly ghost kmsConstructedRegion: Option<string>,
+    nameonly ghost ddbConstructedRegion: Option<string>
+  )
+
+  type InternalConfig = Config
+
+  predicate ValidInternalConfig?(config: InternalConfig)
+  {
+    && true
+
+    // && (config.kmsConfiguration.kmsKeyArn? ==> KmsArn.ValidKmsArn?(config.kmsConfiguration.kmsKeyArn))
+    // && (config.kmsConfiguration.kmsMRKeyArn? ==> KmsArn.ValidKmsArn?(config.kmsConfiguration.kmsMRKeyArn))
+    // && config.kmsClient.ValidState()
+    && config.storage.ValidState()
+       // && config.storage.Modifies !! config.kmsClient.Modifies
+    && (config.storage is DefaultEncryptedKeyStore.DynamoDBEncryptedKeyStore
+        ==>
+          config.logicalKeyStoreName == (config.storage as DefaultEncryptedKeyStore.DynamoDBEncryptedKeyStore).logicalKeyStoreName)
+  }
+
+  function ModifiesInternalConfig(config: InternalConfig) : set<object>
+  {
+    config.storage.Modifies
+  }
+
+
+  predicate CreateKeyEnsuresPublicly(input: CreateKeyInput , output: Result<CreateKeyOutput, Error>)
+  {true}
+
+  method CreateKey ( config: InternalConfig , input: CreateKeyInput )
+    returns (output: Result<CreateKeyOutput, Error>)
+  {
+
+    :- Need(
+      KmsArn.ValidKmsArn?(match input.kmsArn
+                          case kmsKeyArn(kmsKeyArn) => kmsKeyArn
+                          case kmsMRKeyArn(kmsMRKeyArn) => kmsMRKeyArn),
+      Types.KeyStoreAdminException(
+        message := ErrorMessages.CREATE_KEY_STORE_DEPRECATED
+      )
+    );
+
+    match input.kms
+    case ReEncrypt(kmsClient) =>
+
+      assume {:axiom} config.storage.Modifies !! kmsClient.Modifies;
+      assume kmsClient.ValidState();
+
+      var legacyConfig := KeyStoreOperations.Config(
+        id := "",
+        ddbTableName := None,
+        logicalKeyStoreName := config.logicalKeyStoreName,
+        kmsConfiguration := match input.kmsArn
+        case kmsKeyArn(kmsKeyArn) => KeyStoreOperations.Types.kmsKeyArn(kmsKeyArn)
+        case kmsMRKeyArn(kmsMRKeyArn) => KeyStoreOperations.Types.kmsMRKeyArn(kmsMRKeyArn),
+        grantTokens := [],
+        kmsClient := kmsClient,
+        ddbClient := None,
+        storage := config.storage,
+        kmsConstructedRegion := None,
+        ddbConstructedRegion := None
+      );
+
+      assert KeyStoreOperations.ValidInternalConfig?(legacyConfig);
+
+      var output? := KeyStoreOperations.CreateKey(
+        config := legacyConfig,
+        input := KeyStoreOperations.Types.CreateKeyInput(
+          branchKeyIdentifier := input.branchKeyIdentifier,
+          encryptionContext := input.encryptionContext
+        )
+      );
+
+      var value :- output?
+      .MapFailure(e => Types.AwsCryptographyKeyStore(e));
+
+      output := Success(Types.CreateKeyOutput(
+        branchKeyIdentifier := value.branchKeyIdentifier
+      ));
+  }
+
+
+  predicate VersionKeyEnsuresPublicly(input: VersionKeyInput, output: Result<VersionKeyOutput, Error>)
+  {true}
+
+  method VersionKey(config: InternalConfig, input: VersionKeyInput)
+    returns (output: Result<VersionKeyOutput, Error>)
+
+}
